114-minSubArraySum.dfy
@@ -5,28 +5,32 @@ function Sum(a: seq<int>, s: int, t: int): int
 }
 // pure-end
 method minSubArraySum(a: seq<int>) returns (s: int)
+  // pre-conditions-start
+  requires |a| > 0
+  // pre-conditions-end
   // post-conditions-start
-  ensures forall p,q :: 0 <= p <= q <= |a| ==> Sum(a, p, q) >= s
-  ensures exists k, m :: 0 <= k <= m <= |a| && s == Sum(a, k, m)
+  ensures forall p,q :: 0 <= p < q <= |a| ==> Sum(a, p, q) >= s
+  ensures exists k, m :: 0 <= k < m <= |a| && s == Sum(a, k, m)
   // post-conditions-end
 {
   // impl-start
-  var k, m := 0, 0;
-  s := 0;
-  var n := 0;
-  var c, t := 0, 0;
+  var k, m := 0, 1;
+  s := a[0];
+  var n := 1;
+  var c, t := 0, a[0];
   while n < |a|
     // invariants-start
-    invariant 0 <= c <= n <= |a| && t == Sum(a, c, n)
-    invariant forall b :: 0 <= b <= n ==> Sum(a, b, n) >= Sum(a, c, n)
-    invariant 0 <= k <= m <= n && s == Sum(a, k, m)
-    invariant forall p,q :: 0 <= p <= q <= n ==> Sum(a, p, q) >= Sum(a, k, m)
+    invariant 0 <= c < n <= |a| && t == Sum(a, c, n)
+    invariant forall b :: 0 <= b < n ==> Sum(a, b, n) >= Sum(a, c, n)
+    invariant 0 <= k < m <= n && s == Sum(a, k, m)
+    invariant forall p,q :: 0 <= p < q <= n ==> Sum(a, p, q) >= Sum(a, k, m)
     // invariants-end
   {
     t, n := t + a[n], n + 1;
-    if t > 0 {
-      c, t := n, 0;
-    } else if s > t {
+    if t > a[n - 1] {
+      c, t := n - 1, a[n - 1];
+    }
+    if s > t {
       k, m, s := c, n, t;
     }
   }
