127-intersection.dfy
@@ -14,7 +14,7 @@ function max(a: int, b: int): int
   if a >= b then a else b
 }
 // pure-end
-method Intersection(start1: int, end1: int, start2: int, end2: int) returns (result: string)
+method intersection(start1: int, end1: int, start2: int, end2: int) returns (result: string)
   // pre-conditions-start
   requires start1 <= end1 && start2 <= end2
   // pre-conditions-end
@@ -38,19 +38,4 @@ method Intersection(start1: int, end1: int, start2: int, end2: int) returns (res
 
   return "NO";
   // impl-end
-}
-
-method {:test} Main()
-{
-  var result1 := Intersection(1, 2, 2, 3);
-  assert result1 == "NO";
-
-  var result2 := Intersection(-1, 1, 0, 4);
-  // The intersection is [0, 1], which has length 2, a prime number
-  assert result2 == "YES";
-
-  var result3 := Intersection(-3, -1, -5, 5);
-  assert result3 == "YES";
-
-  print "All tests passed!\n";
 }
