132-is_nested.dfy
@@ -1,6 +1,9 @@
-method is_nested(s: seq<int>) returns (res: bool) 
+method is_nested(s: string) returns (res: bool)
+    // pre-conditions-start
+    requires forall i :: 0 <= i < |s| ==> s[i] == '[' || s[i] == ']'
+    // pre-conditions-end
     // post-conditions-start
-    ensures res == exists x, y, z, w :: 0 <= x < y < z < w < |s| && s[x] == 0 && s[y] == 0 && s[z] == 1 && s[w] == 1
+    ensures res == exists x, y, z, w :: 0 <= x < y < z < w < |s| && s[x] == '[' && s[y] == '[' && s[z] == ']' && s[w] == ']'
     // post-conditions-end
 {
     // impl-start
@@ -10,12 +13,12 @@ method is_nested(s: seq<int>) returns (res: bool)
     while i < |s| && bal < 2
         // invariants-start
         invariant 0 <= i <= |s|
-        invariant (bal >= 1) == (exists x :: 0 <= x < i && s[x] == 0)
-        invariant (bal >= 2) == (exists x, y :: 0 <= x < y < i && s[x] == 0 && s[y] == 0)
-        invariant !(exists x, y, z :: 0 <= x < y < z < i && s[x] == 0 && s[y] == 0 && s[z] == 1)
+        invariant (bal >= 1) == (exists x :: 0 <= x < i && s[x] == '[')
+        invariant (bal >= 2) == (exists x, y :: 0 <= x < y < i && s[x] == '[' && s[y] == '[')
+        invariant !(exists x, y, z :: 0 <= x < y < z < i && s[x] == '[' && s[y] == '[' && s[z] == ']')
         // invariants-end
     {
-        if s[i] == 0 {
+        if s[i] == '[' {
             bal := bal + 1;
         }
         i := i + 1;
@@ -29,12 +32,12 @@ method is_nested(s: seq<int>) returns (res: bool)
         // invariants-start
         invariant 0 <= i <= |s|
         invariant 0 <= bal <= 2
-        invariant exists x, y :: 0 <= x && x < y && y < i && s[x] == 0 && s[y] == 0
-        invariant (bal <= 1) == (exists x, y, z :: 0 <= x < y < z < i && s[x] == 0 && s[y] == 0 && s[z] == 1)
-        invariant (bal == 0) == (exists x, y, z, w :: 0 <= x < y < z < w < i && s[x] == 0 && s[y] == 0 && s[z] == 1 && s[w] == 1)
+        invariant exists x, y :: 0 <= x && x < y && y < i && s[x] == '[' && s[y] == '['
+        invariant (bal <= 1) == (exists x, y, z :: 0 <= x < y < z < i && s[x] == '[' && s[y] == '[' && s[z] == ']')
+        invariant (bal == 0) == (exists x, y, z, w :: 0 <= x < y < z < w < i && s[x] == '[' && s[y] == '[' && s[z] == ']' && s[w] == ']')
         // invariants-end
     {
-        if s[i] == 1 {
+        if s[i] == ']' {
             bal := bal - 1;
         }
         i := i + 1;
